PERF switching from gmap to avl trees
- the fixes a significant performance regression on large files

theories/bytestring.v
@@ -7,6 +7,7 @@ Require Import Coq.Strings.String.
 Require Import stdpp.countable.
 
 Set Primitive Projections.
+Set Default Proof Using "Type".
 
 (** bytes *)
 Instance byte_dec : EqDecision Byte.byte := Byte.byte_eq_dec.
@@ -160,3 +161,193 @@ Local Fixpoint contains (start: nat) (keys: list bs) (fullname: bs) :bool :=
 
 Definition eqb (a b : bs) : bool :=
   if decide (a = b) then true else false.
+
+Definition byte_cmp (a b : Byte.byte) : comparison :=
+  N.compare (Byte.to_N a) (Byte.to_N b).
+
+
+(** comparison *)
+Require Import Coq.Structures.OrderedType.
+
+Lemma to_N_inj : forall x y, Byte.to_N x = Byte.to_N y <-> x = y.
+Proof.
+  split.
+  2: destruct 1; reflexivity.
+  intros.
+  assert (Some x = Some y).
+  { do 2 rewrite <- Byte.of_to_N.
+    destruct H. reflexivity. }
+  injection H0. auto.
+Qed.
+
+Module OT_byte <: OrderedType.OrderedType with Definition t := Byte.byte.
+  Definition t := Byte.byte.
+  Definition eq := fun l r => byte_cmp l r = Eq.
+  Definition lt := fun l r => byte_cmp l r = Lt.
+  Theorem eq_refl : ∀ x : t, eq x x.
+  Proof.
+    intros; apply N.compare_refl.
+  Qed.
+  Theorem eq_sym : ∀ x y : t, eq x y → eq y x.
+  Proof.
+    intros. eapply N.compare_eq in H. red. unfold byte_cmp.
+    destruct H. apply eq_refl.
+  Qed.
+  Theorem eq_trans : ∀ x y z : t, eq x y → eq y z → eq x z.
+  Proof.
+    intros. eapply N.compare_eq in H. eapply N.compare_eq in H0.
+    red. unfold byte_cmp.
+    destruct H. destruct H0. apply eq_refl.
+  Qed.
+  Theorem lt_trans : ∀ x y z : t, lt x y → lt y z → lt x z.
+  Proof.
+    unfold lt, byte_cmp.
+    intros.
+    rewrite N.compare_lt_iff in H.
+    rewrite N.compare_lt_iff in H0.
+    rewrite N.compare_lt_iff.
+    lia.
+  Qed.
+  Theorem lt_not_eq : ∀ x y : t, lt x y → ¬ eq x y.
+  Proof.
+    unfold lt, eq, byte_cmp; intros.
+    rewrite N.compare_lt_iff in H.
+    rewrite N.compare_eq_iff.
+    lia.
+  Qed.
+  Definition compare (x y : t) : OrderedType.Compare lt eq x y.
+    refine  (
+    match byte_cmp x y as X return byte_cmp x y = X -> OrderedType.Compare lt eq x y  with
+    | Eq => fun pf => OrderedType.EQ pf
+    | Lt => fun pf => OrderedType.LT pf
+    | Gt => fun pf => OrderedType.GT _
+    end (Logic.eq_refl)).
+    unfold lt, byte_cmp.
+    rewrite N.compare_antisym.
+    apply CompOpp_iff. apply pf.
+  Defined.
+
+  Definition eq_dec : ∀ x y : t, {eq x y} + {¬ eq x y}.
+  refine (fun x y =>
+      match byte_cmp x y as Z return byte_cmp x y = Z -> _ with
+      | Eq => fun pf => left pf
+      | _ => fun _ => right _
+      end Logic.eq_refl).
+  unfold eq. congruence.
+  unfold eq. congruence.
+  Defined.
+
+End OT_byte.
+
+Fixpoint bs_cmp (xs ys : bs) : comparison :=
+  match xs , ys with
+  | Bytestring.EmptyString , Bytestring.EmptyString => Eq
+  | Bytestring.EmptyString , _ => Lt
+  | _ , Bytestring.EmptyString => Gt
+  | Bytestring.String x xs , Bytestring.String y ys =>
+    match byte_cmp x y with
+    | Eq => bs_cmp xs ys
+    | x => x
+    end
+  end%bs.
+
+Lemma byte_cmp_refl : forall a, byte_cmp a a = Eq.
+Proof.
+  intros. unfold byte_cmp.
+  eapply N.compare_refl.
+Defined.
+
+Theorem byte_cmp_spec : forall x y, CompareSpec (x = y) (OT_byte.lt x y) (OT_byte.lt y x) (byte_cmp x y).
+Proof.
+  intros. unfold byte_cmp.
+  unfold OT_byte.lt, byte_cmp.
+  destruct (N.compare_spec (Byte.to_N x) (Byte.to_N y)); constructor; auto.
+  apply to_N_inj. assumption.
+Qed.
+
+
+Module OT_bs <: OrderedType.OrderedType with Definition t := bs.
+  Definition t := bs.
+  Definition eq := @eq bs.
+  Definition lt := fun l r => bs_cmp l r = Lt.
+
+  Theorem lm : forall x y, CompareSpec (x = y) (lt x y) (lt y x) (bs_cmp x y).
+  Proof.
+    induction x; destruct y; simpl.
+    - constructor; reflexivity.
+    - constructor. reflexivity.
+    - constructor. reflexivity.
+    - unfold lt; simpl.
+      destruct (byte_cmp_spec b b0); simpl.
+      + subst. destruct (IHx y); constructor; eauto.
+        congruence.
+        destruct (byte_cmp_spec b0 b0); try congruence.
+        red in H0. rewrite OT_byte.eq_refl in H0. congruence.
+      + constructor; auto.
+      + red in H. rewrite H. constructor; auto.
+  Qed.
+
+  Definition compare (x y : t) : OrderedType.Compare lt eq x y.
+    refine  (
+    match bs_cmp x y as X return bs_cmp x y = X -> OrderedType.Compare lt eq x y  with
+    | Eq => fun pf => OrderedType.EQ _
+    | Lt => fun pf => OrderedType.LT pf
+    | Gt => fun pf => OrderedType.GT _
+    end (Logic.eq_refl)).
+    generalize (lm x y). rewrite pf. inversion 1; auto.
+    generalize (lm x y). rewrite pf. inversion 1; auto.
+  Defined.
+
+  Theorem eq_refl : ∀ x : t, eq x x.
+  Proof.
+    reflexivity.
+  Qed.
+  Theorem eq_sym : ∀ x y : t, eq x y → eq y x.
+  Proof.
+    eapply eq_sym.
+  Qed.
+  Theorem eq_trans : ∀ x y z : t, eq x y → eq y z → eq x z.
+  Proof.
+    eapply eq_trans.
+  Qed.
+  Theorem lt_trans : ∀ x y z : t, lt x y → lt y z → lt x z.
+  Proof.
+    unfold lt.
+    induction x; destruct y; simpl; try congruence.
+    - destruct z; congruence.
+    - destruct (byte_cmp_spec b b0); subst.
+      + destruct z; auto.
+        destruct (byte_cmp b0 b); auto.
+        eauto.
+      + destruct z; auto.
+        red in H.
+        destruct (byte_cmp b0 b1) eqn:?.
+        * generalize (byte_cmp_spec b0 b1).
+          rewrite Heqc. inversion 1.
+          subst. rewrite H. auto.
+        * generalize (OT_byte.lt_trans _ _ _ H Heqc). unfold OT_byte.lt.
+          intro X; rewrite X. auto.
+        * congruence.
+      + congruence.
+  Qed.
+  Theorem lt_not_eq : ∀ x y : t, lt x y → ¬ eq x y.
+  Proof.
+    unfold lt, eq.
+    intros. intro. subst.
+    induction y; simpl in *; try congruence.
+    rewrite byte_cmp_refl in *. auto.
+  Qed.
+
+  Definition eq_dec : ∀ x y : t, {eq x y} + {¬ eq x y}.
+  refine (fun x y =>
+      match bs_cmp x y as Z return CompareSpec _ _ _ Z -> _ with
+      | Eq => fun pf => left _
+      | _ => fun _ => right _
+      end (lm x y)).
+  - inversion pf. apply H.
+  - apply lt_not_eq. inversion c. auto.
+  - inversion c. apply lt_not_eq in H.
+    unfold eq in *. congruence.
+  Defined.
+
+End OT_bs.
