theories/avl.v
@@ -1,0 +1,167 @@
+(*
+ * Copyright (C) BedRock Systems Inc. 2019-2020 Gregory Malecha
+ *
+ * SPDX-License-Identifier:AGPL-3.0-or-later
+ *)
+Require Import stdpp.gmap.
+Require Import bedrock.bytestring.
+
+Require Import Coq.FSets.FMapAVL.
+
+Set Default Proof Using "Type".
+
+Module IM := FMapAVL.Make OT_bs.
+
+Instance IMR_lookup {V} : Lookup bs V (IM.Raw.t V) :=
+  @IM.Raw.find _.
+
+Instance IMR_empty {V} : Empty (IM.Raw.t V) :=
+  @IM.Raw.empty _.
+
+Instance IMR_insert {V} : Insert bs V (IM.Raw.t V) :=
+  @IM.Raw.add _.
+
+Instance IMR_map : FMap IM.Raw.t := @IM.Raw.map.
+
+Instance IMR_merge : Merge IM.Raw.t := IM.Raw.map2.
+
+Instance IMR_maptolist : FinMapToList bs A (IM.Raw.t A) := IM.Raw.elements.
+
+Instance IMR_singleton {V} : SingletonM bs V (IM.Raw.t V) :=
+  fun k v => <[ k := v ]> ∅.
+
+
+
+Instance IM_lookup {V} : Lookup bs V (IM.t V) :=
+  @IM.find _.
+
+Instance IM_empty {V} : Empty (IM.t V) :=
+  @IM.empty _.
+
+Instance IM_insert {V} : Insert bs V (IM.t V) :=
+  @IM.add _.
+
+Instance IM_map : FMap IM.t := @IM.map.
+
+Instance IM_merge : Merge IM.t := IM.map2.
+
+Instance IM_maptolist : FinMapToList bs A (IM.t A) := IM.elements.
+
+Instance IM_singleton {V} : SingletonM bs V (IM.t V) :=
+  fun k v => <[ k := v ]> ∅.
+
+Definition find_any {T} (b : bs -> T -> bool) (l : IM.t T) : bool :=
+  IM.fold (λ (k : IM.key) (v : T) (acc : bool), if acc then true else b k v) l false.
+
+Theorem find_any_ok : forall {T} b (l : IM.t T),
+    if find_any b l then
+      exists k v, IM.MapsTo k v l /\ b k v = true
+    else
+      forall k v, IM.MapsTo k v l -> b k v = false.
+Proof.
+  unfold find_any.
+  intros. rewrite IM.fold_1.
+  assert (if
+   fold_left (λ (a : bool) (p : IM.key * T), if a then true else b p.1 p.2)
+     (IM.elements (elt:=T) l) false
+  then ∃ (k : IM.key) (v : T), SetoidList.InA (IM.eq_key_elt (elt:=T)) (k, v) (IM.elements l) ∧ b k v = true
+  else ∀ (k : IM.key) (v : T), SetoidList.InA (IM.eq_key_elt (elt:=T)) (k, v) (IM.elements l) → b k v = false).
+  { induction (IM.elements l); simpl; intros.
+    { inversion H. }
+    { destruct (b a.1 a.2) eqn:?.
+      { enough (fold_left (λ (a0 : bool) (p : IM.key * T), if a0 then true else b p.1 p.2) l0 true = true) as ->.
+        { do 2 eexists. split; eauto. left. split; reflexivity. }
+        clear. induction l0; simpl; auto. }
+      { destruct (fold_left (λ (a : bool) (p : IM.key * T), if a then true else b p.1 p.2) l0
+            false).
+        { destruct IHl0 as [ ? [ ? [ ? ? ] ] ].
+          do 2 eexists; split; eauto. }
+        { intros. inversion H; subst.
+          { inversion H1; simpl in *; subst; auto. }
+          { eauto. } } } } }
+  { destruct (fold_left (λ (a : bool) (p : IM.key * T), if a then true else b p.1 p.2)
+                        (IM.elements (elt:=T) l) false).
+    { destruct H as [ k [ v [ ? ? ] ] ].
+      do 2 eexists; split; eauto using IM.elements_2. }
+    { intros. apply H. eauto using IM.elements_1. } }
+Qed.
+
+Fixpoint check_canon {e} (min max : option bs) (b : IM.Raw.tree e) : bool.
+destruct b.
+- apply true.
+- refine (check_canon _ min (Some k) b1 &&
+          check_canon _ (Some k) max b2 &&
+          match min with
+          | None => true
+          | Some m => match bs_cmp m k with
+                     | Lt => true
+                     | _ => false
+                     end
+          end &&
+          match max with
+          | None => true
+          | Some m => match bs_cmp k m with
+                     | Lt => true
+                     | _ => false
+                     end
+          end).
+Defined.
+
+Local Lemma check_canon_lem : forall e (b : IM.Raw.tree e) min max,
+    check_canon min max b ->
+    IM.Raw.bst b /\
+    match min with
+    | None => True
+    | Some m => IM.Raw.gt_tree m b
+    end /\
+    match max with
+    | None => True
+    | Some m => IM.Raw.lt_tree m b
+    end.
+Proof.
+  induction b; simpl; intros.
+  { repeat constructor.
+    - destruct min; repeat constructor.
+      red. inversion 1.
+    - destruct max; repeat constructor.
+      red. inversion 1. }
+  {  repeat match goal with
+           | H : Is_true (_ && _) |- _ => eapply andb_prop_elim in H; destruct H
+           end.
+     specialize (IHb2 _ _ H2).
+     specialize (IHb1 _ _ H).
+     simpl in *.
+     repeat match goal with
+            | H : _ /\ _ |- _ => destruct H
+            end.
+     repeat constructor; eauto.
+     { destruct min; simpl in *; auto.
+       red. inversion 1; subst.
+       { destruct (bs_cmp b k); simpl in *; try congruence; contradiction. }
+       { apply H7 in H11. auto. }
+       { apply H4 in H11.
+         destruct (bs_cmp b k) eqn:?; simpl in *; try contradiction.
+         eapply IM.E.lt_trans; eauto. } }
+     { destruct max; simpl in *; auto.
+       red. inversion 1; subst.
+       { destruct (bs_cmp k b); simpl in *; try congruence; contradiction. }
+       { apply H8 in H11.
+         destruct (bs_cmp k b) eqn:?; simpl in *; try contradiction.
+         eapply IM.E.lt_trans; eauto. }
+       { apply H5; auto. } } }
+Qed.
+
+Theorem check_canon_ok : forall e (b : IM.Raw.tree e), check_canon None None b -> IM.Raw.bst b.
+Proof.
+  intros. apply check_canon_lem in H. tauto.
+Qed.
+
+Definition build {e} (b : IM.Raw.t e) (pf : Is_true (check_canon None None b)) :IM.t e :=
+  {| IM.this := b; IM.is_bst := check_canon_ok _ _ pf |}.
+
+(* this canonicalizes the proof *)
+Definition map_canon {e} (b : IM.t e) : IM.t e :=
+  match check_canon None None b.(IM.this) as X return (X -> IM.Raw.bst b.(IM.this)) -> _ with
+  | true => fun x => {| IM.this := IM.this b; IM.is_bst := x I |}
+  | false => fun _ => b
+  end (@check_canon_ok _ b.(IM.this)).
