theories/lang/cpp/parser.v
@@ -10,6 +10,8 @@ Require Export
 Require Import stdpp.gmap.
 Require Export bedrock.lang.cpp.ast.
 
+Set Default Proof Using "Type".
+
 Definition Nanon (ty : globname) : globname :=
   ("#" ++ ty)%bs.
 
@@ -30,159 +32,73 @@ Notation "` e `" := e (e custom cppglobal at level 200, at level 0) : cppfield_s
 
 (** this is the compatibility layer, cpp2v generates these definitions
  *)
-(* HACK to get around the fact that [gmap_empty] is opaque. *)
-Local Definition empty_symbols : symbol_table :=
-  Eval vm_compute in gmap_empty.
-Local Definition empty_globals : type_table :=
-  Eval vm_compute in gmap_empty.
-Local Instance symbol_table_empty_trans : Empty symbol_table := empty_symbols.
-Local Instance type_table_empty_trans : Empty type_table := empty_globals.
+Definition translation_unitK : Type :=
+  symbol_table -> type_table -> (symbol_table -> type_table -> translation_unit) -> translation_unit.
 
-Definition Dvar (name : obj_name) (t : type) (init : option Expr) : translation_unit :=
-  {| symbols := {[ name := Ovar t init ]}
-   ; globals := ∅ |}.
+Definition Dvar (name : obj_name) (t : type) (init : option Expr) : translation_unitK :=
+  fun syms tys k => k (<[ name := Ovar t init ]> syms) tys.
 
-Definition Dfunction    (name : obj_name) (f : Func) : translation_unit :=
-  {| symbols := {[ name := Ofunction f ]}
-   ; globals := ∅ |}.
-Definition Dmethod    (name : obj_name) (f : Method) : translation_unit :=
-  {| symbols := {[ name := Omethod f ]}
-   ; globals := ∅ |}.
-Definition Dconstructor    (name : obj_name) (f : Ctor) : translation_unit :=
-  {| symbols := {[ name := Oconstructor f ]}
-   ; globals := ∅ |}.
-Definition Ddestructor    (name : obj_name) (f : Dtor) : translation_unit :=
-  {| symbols := {[ name := Odestructor f ]}
-   ; globals := ∅ |}.
-Definition Dunion (name : globname) (o : option Union) : translation_unit :=
-  {| symbols := ∅
-   ; globals := {[ name := match o with
-                           | None => Gtype
-                           | Some u => Gunion u
-                           end ]} |}.
-Definition Dstruct (name : globname) (o : option Struct) : translation_unit :=
-  {| symbols := ∅
-   ; globals := {[ name := match o with
-                           | None => Gtype
-                           | Some u => Gstruct u
-                           end ]} |}.
+Definition Dfunction    (name : obj_name) (f : Func) : translation_unitK :=
+  fun syms tys k => k (<[ name := Ofunction f ]> syms) tys.
+Definition Dmethod    (name : obj_name) (f : Method) : translation_unitK :=
+  fun syms tys k => k (<[ name := Omethod f ]> syms) tys.
+Definition Dconstructor    (name : obj_name) (f : Ctor) : translation_unitK :=
+  fun syms tys k => k (<[ name := Oconstructor f ]> syms) tys.
+Definition Ddestructor    (name : obj_name) (f : Dtor) : translation_unitK :=
+  fun syms tys k => k (<[ name := Odestructor f ]> syms) tys.
 
-Definition Denum (name : globname) (t : option type) (branches : list (ident * BinNums.Z)) : translation_unit :=
-  {| symbols := ∅
-   ; globals :=
-       let enum_ty := Tnamed name in
-       let raw_ty :=
-           match t with
-           | None => enum_ty
-           | Some t => t
-           end
-       in
-       match t with
-       | Some t => {[ name := Genum t (List.map fst branches) ]}
-       | None => ∅
-       end ∪
-       list_to_map (List.map (fun '(nm, oe) => (nm, Gconstant enum_ty (Some (Eint oe raw_ty)))) branches) |}.
+Definition Dunion (name : globname) (o : option Union) : translation_unitK :=
+  fun syms tys k =>
+    k syms (<[ name := match o with
+                       | None => Gtype
+                       | Some u => Gunion u
+                       end ]> tys).
+Definition Dstruct (name : globname) (o : option Struct) : translation_unitK :=
+  fun syms tys k =>
+    k syms (<[ name := match o with
+                       | None => Gtype
+                       | Some u => Gstruct u
+                       end ]> tys).
+
+Definition Denum (name : globname) (t : option type) (branches : list (ident * BinNums.Z)) : translation_unitK :=
+  fun syms tys k =>
+    let enum_ty := Tnamed name in
+    let raw_ty :=
+        match t with
+        | None => enum_ty
+        | Some t => t
+        end
+    in
+    k syms (List.fold_left (fun acc '(nm, oe) => <[ nm := Gconstant enum_ty (Some (Eint oe raw_ty)) ]> acc) 
+                           branches
+                           match t with
+                           | Some t => <[ name := Genum t (List.map fst branches) ]> tys
+                           | None => tys
+                           end).
   (* ^ enumerations (the initializers need to be constant expressions) *)
 
-Definition Dconstant    (name : globname) (t : type) (e : Expr) : translation_unit :=
-  {| symbols := ∅
-   ; globals := {[ name := Gconstant t (Some e) ]} |}.
-Definition Dconstant_undef  (name : globname) (t : type) : translation_unit :=
-  {| symbols := ∅
-   ; globals := {[ name := Gconstant t None ]} |}.
-Definition Dtypedef     (name : globname) (t : type) : translation_unit :=
-  {| symbols := ∅
-   ; globals := {[ name := Gtypedef t ]} |}.
-Definition Dtype (name : globname) : translation_unit :=
-  {| symbols := ∅
-   ; globals := {[ name := Gtype ]}|}.
+Definition Dconstant    (name : globname) (t : type) (e : Expr) : translation_unitK :=
+  fun syms tys k => k syms (<[ name := Gconstant t (Some e) ]> tys).
+Definition Dconstant_undef  (name : globname) (t : type) : translation_unitK :=
+  fun syms tys k => k syms (<[ name := Gconstant t None ]> tys).
+Definition Dtypedef     (name : globname) (t : type) : translation_unitK :=
+  fun syms tys k => k syms (<[ name := Gtypedef t ]> tys).
+Definition Dtype (name : globname) : translation_unitK :=
+  fun syms tys k => k syms (<[ name := Gtype ]> tys).
+Definition translation_unit_canon (c : translation_unit) : translation_unit :=
+  {| symbols := avl.map_canon c.(symbols)
+   ; globals := avl.map_canon c.(globals) |}.
 
-
-Definition Is_true_canon {b} : Is_true b -> Is_true b :=
-  match b as b return Is_true b -> Is_true b with
-  | true => fun _ => I
-  | false => fun pf => match pf with end
-  end.
-
-Require stdpp.pmap.
-
-Definition pmap_canon {K} (s : pmap.Pmap K) : pmap.Pmap K.
-destruct s.
-exists pmap_car. apply Is_true_canon. assumption.
-Defined.
-
-Definition stringmap_canon {K} (s : gmap bs K) : gmap bs K.
-  destruct s.
-  refine (
-      let t := bool_decide
-           (map_Forall
-              (λ (p : positive) (_ : K),
-                 countable.encode <$> countable.decode p = Some p)
-              (pmap_canon gmap_car)) in
-match t as X return X = t -> _ with
-| true => _
-| false => _
-end eq_refl
-).
-{ exists (pmap_canon gmap_car).
-  red. apply Is_true_canon.
-  subst t. red. rewrite <- H. exact I. }
-{ exists gmap_car. apply Is_true_canon. assumption. }
-Defined.
-
-Definition compilation_union_canon (c : translation_unit) : translation_unit :=
-  {| symbols := stringmap_canon c.(symbols)
-   ; globals := stringmap_canon c.(globals) |}.
-
-Fixpoint decls' (ls : list translation_unit) : translation_unit :=
+Fixpoint decls' (ls : list translation_unitK) : translation_unitK :=
   match ls with
-  | nil => {| symbols := ∅ ; globals := ∅ |}
-  | m :: ms =>
-    let res := decls' ms in
-    {| symbols := m.(symbols) ∪ res.(symbols)
-     ; globals := m.(globals) ∪ res.(globals) |}
+  | nil => fun syms tys k => k syms tys
+  | m :: ms => fun syms tys k => m syms tys (fun s t => decls' ms s t k)
   end.
 
 Definition decls ls : translation_unit :=
-  compilation_union_canon (decls' ls).
+  decls' ls ∅ ∅ (fun a b => {| symbols := avl.map_canon a
+                           ; globals := avl.map_canon b |}).
 
-Declare Reduction reduce_translation_unit :=
-  cbv beta iota zeta delta
-      [ decls decls' compilation_union_canon pmap_canon pmap.Pmap_wf andb
-        parser.empty_globals parser.empty_symbols
-        Dvar Dfunction Dmethod Dconstructor Ddestructor
-        Dunion Dstruct Denum Dconstant Dconstant_undef Dtypedef Dtype
-        stringmap_canon symbols globals
-        union map_union union_with map_union_with merge gmap.gmap_merge
-        pmap.Pmerge pmap.Pmerge_raw pmap.Pomap_raw
-        singletonM map_singleton
-        insert map_insert
-        partial_alter gmap.gmap_partial_alter pmap.Ppartial_alter pmap.Ppartial_alter_raw
-        countable.encode
-        option_union_with byte_countable
-        Bytestring.print Bytestring.parse Bytestring.t_dec bytestring_countable bytestring.append
-        Papp
-        empty pmap.Psingleton_raw flip mbind compose option_bind
-        pmap.PNode'
-        List.map fst snd
-        list_to_map
-        names.globname_eq
-        names.localname_eq
-        names.ident_eq
-        names.obj_name_eq
-        string_rec string_rect decide_rel
-        negb
-        foldr Ascii.shift
-
-        symbol_table_empty_trans type_table_empty_trans parser.empty_symbols parser.empty_globals
-
-        list_countable
-        option_ret option_bind mret mbind mapM list_rect list_fmap list_eq_dec
-        positives_flatten N_countable positives_unflatten positives_flatten_go Byte.to_N Byte.of_N
-
-positives_unflatten_go Pdup Pos.succ
-Pos.pred_N Pos.pred_double
-
-        Is_true_canon bool_decide map_Forall_dec map_to_list decide curry pmap.Pto_list list.Forall_dec list.Forall_Exists_dec countable.decode shift pmap.Pto_list_raw from_option List.app curry_dec Preverse decide_rel option_eq_dec fmap option_fmap option_map numbers.positive_eq_dec Pos.eq_dec positive_rec positive_rect Preverse_go sumbool_rect sumbool_rec ].
+Declare Reduction reduce_translation_unit := vm_compute.
 
 Export Bytestring.
